Sq a b -> sq a

code/ecdsap256sha2/Hacl.Impl.P256.MontgomeryMultiplication.fst
@@ -190,17 +190,17 @@ let montgomery_multiplication_buffer a b result =
   pop_frame()  
 
 
-val montgomery_square_buffer: a: felem -> b: felem -> result: felem ->  Stack unit
-  (requires (fun h -> live h a /\ as_nat h a < prime256 /\ live h b /\ live h result /\ as_nat h b < prime256)) 
+val montgomery_square_buffer: a: felem -> result: felem ->  Stack unit
+  (requires (fun h -> live h a /\ as_nat h a < prime256 /\ live h result)) 
   (ensures (fun h0 _ h1 -> 
     modifies (loc result) h0 h1 /\  
-    as_nat h1 result = (as_nat h0 a * as_nat h0 b * modp_inv2_prime (pow2 256) prime256) % prime256 /\
-    as_nat h1 result = toDomain_ (fromDomain_ (as_nat h0 a) * fromDomain_ (as_nat h0 b) % prime256) /\
-    as_nat h1 result = toDomain_ (fromDomain_ (as_nat h0 a) * fromDomain_ (as_nat h0 b)))
+    as_nat h1 result = (as_nat h0 a * as_nat h0 a * modp_inv2_prime (pow2 256) prime256) % prime256 /\
+    as_nat h1 result = toDomain_ (fromDomain_ (as_nat h0 a) * fromDomain_ (as_nat h0 a) % prime256) /\
+    as_nat h1 result = toDomain_ (fromDomain_ (as_nat h0 a) * fromDomain_ (as_nat h0 a)))
   )
 
 
-let montgomery_square_buffer a b result = 
+let montgomery_square_buffer a result = 
   assert_norm(prime256 > 3);
   push_frame();
     let t = create (size 8) (u64 0) in 
@@ -209,7 +209,7 @@ let montgomery_square_buffer a b result =
       let h0 = ST.get() in 
     sq a t;  
       let h1 = ST.get() in 
-      mul_lemma_ (as_nat h0 a) (as_nat h0 b) prime256;
+      mul_lemma_ (as_nat h0 a) (as_nat h0 a) prime256;
   montgomery_multiplication_round_twice t round2;
       let h2 = ST.get() in 
   montgomery_multiplication_round_twice round2 round4; 
@@ -218,7 +218,7 @@ let montgomery_square_buffer a b result =
   lemma_mod_mul_distr_l (wide_as_nat h2 round2) (modp_inv2_prime (pow2 128) prime256) prime256;
   lemma_mod_mul_distr_l (wide_as_nat h1 t * modp_inv2_prime (pow2 128) prime256) (modp_inv2_prime (pow2 128) prime256) prime256;
       mul_lemma_2 (wide_as_nat h1 t % pow2 64) (pow2 64 - 1) prime256;
-      mul_lemma_ (as_nat h0 a) (as_nat h0 b) prime256;
+      mul_lemma_ (as_nat h0 a) (as_nat h0 a) prime256;
       mul_lemma_1 ( 
          let round = (wide_as_nat h1 t + prime256 * (wide_as_nat h1 t % pow2 64)) / pow2 64 in  
    round % pow2 64) (pow2 64) prime256; 
@@ -234,12 +234,9 @@ let montgomery_square_buffer a b result =
       assert_norm((prime256 * pow2 64 + (prime256 * pow2 64 + (prime256 * pow2 64 + ((pow2 64 - 1) * prime256 + prime256 * prime256) / pow2 64) / pow2 64)/ pow2 64) / pow2 64 < 2 * prime256);
   reduction_prime256_2prime256_8_with_carry_impl round4 result; 
   lemmaFromDomainToDomain (as_nat h0 a);
-  lemmaFromDomainToDomain (as_nat h0 b);
-  multiplicationInDomainNat #(fromDomain_ (as_nat h0 a)) #(fromDomain_ (as_nat h0 b))  (as_nat h0 a) (as_nat h0 b);
-  inDomain_mod_is_not_mod (fromDomain_ (as_nat h0 a) * fromDomain_ (as_nat h0 b));
+  multiplicationInDomainNat #(fromDomain_ (as_nat h0 a)) #(fromDomain_ (as_nat h0 a))  (as_nat h0 a) (as_nat h0 a);
+  inDomain_mod_is_not_mod (fromDomain_ (as_nat h0 a) * fromDomain_ (as_nat h0 a));
   pop_frame()  
-
-
 
 
 #reset-options "--z3rlimit 500" 
